src/tls/Extensions.fst
@@ -32,6 +32,7 @@ and earlyDataIndication =
    as listed in the RFC's Section 8.2. Labels in the variants below are: 
      M  - "MUST implement"
      AF - "MUST ... when offering applicable features" *)
+
 and extension =
   | E_server_name of list TI.serverName (* M, AF *) (* RFC 6066 *)
 (*| E_max_fragment_length 
@@ -153,7 +154,7 @@ and extensionPayloadBytes role ext =
   | E_supported_groups(l)      -> Parse.namedGroupsBytes l  
   | E_signature_algorithms sha -> sigHashAlgsBytes sha
   | E_key_share ks             -> CommonDH.keyShareBytes ks
-  | E_pre_shared_key psk       -> PSK.preSharedKeyBytes psk
+  | E_pre_shared_key psk -> admit() //PSK.preSharedKeyBytes psk //17-04-21 TODO parse/format the list with ota
   | E_early_data edt           -> earlyDataIndicationBytes edt
   | E_cookie c                 -> c // SI: check 
   | E_supported_versions vv    -> 
@@ -311,7 +312,7 @@ let rec parseExtension role b =
           Correct(E_unknown_extension(head,data))
 	| (0x00z, 0x29z) -> // head TBD, pre shared key
 	  if length data >= 2 then
-	  (match PSK.parsePreSharedKey data with
+	  (match admit() (* 17-04-21 TODO PSK.parsePreSharedKey data *) with
 	  | Correct(psk) -> Correct (E_pre_shared_key psk)
 	  | Error(z) -> Error(z))
 	  else Error (AD_decode_error, perror __SOURCE_FILE__ __LINE__ (err_msg "pre shared key"))
